src/Distributions/DiscreteLaplace/Equivalence.dfy
@@ -1,0 +1,57 @@
+/*******************************************************************************
+ *  Copyright by the contributors to the Dafny Project
+ *  SPDX-License-Identifier: MIT
+ *******************************************************************************/
+
+module DiscreteLaplace.Equivalence {
+  import Rand
+  import Monad
+  import Rationals
+  import BernoulliExpNeg
+  import Uniform
+  import Coin
+  import Model
+
+  /************
+   Definitions
+  ************/
+
+  ghost function SampleTailRecursive(scale: Rationals.Rational, b: bool := true, y: int := 0): Monad.Hurd<int>
+    requires scale.numer >= 1
+  {
+    assume {:axiom} false; // assume termination
+    (s: Rand.Bitstream) =>
+      if !(b && y == 0) then
+        Monad.Result(if b then -y else y, s)
+      else
+        var (u, s) :- Uniform.Model.Sample(scale.numer)(s);
+        var (d, s) :- BernoulliExpNeg.Model.Sample(Rationals.Rational(u, scale.numer))(s);
+        if d then
+          var (v, s) :- SampleTailRecursiveHelper()(s);
+          var x := u + scale.numer * v;
+          var y := x / scale.denom;
+          var sample := Coin.Model.Sample(s);
+          SampleTailRecursive(scale, sample.value, y)(sample.rest)
+        else
+          SampleTailRecursive(scale, b, y)(s)
+
+  }
+
+  ghost function SampleTailRecursiveHelper(a: bool := true, v: int := 0): Monad.Hurd<int> {
+    assume {:axiom} false; // assume termination
+    (s: Rand.Bitstream) =>
+      if !a then
+        Monad.Result(v, s)
+      else
+        var (a, s) :- BernoulliExpNeg.Model.Sample(Rationals.Int(1))(s);
+        SampleTailRecursiveHelper(a, if a then v + 1 else v)(s)
+  }
+
+  /*******
+   Lemmas
+  *******/
+
+  lemma {:axiom} SampleTailRecursiveEquivalence(scale: Rationals.Rational, s: Rand.Bitstream)
+    requires scale.numer >= 1
+    ensures SampleTailRecursive(scale)(s) == Model.Sample(scale)(s)
+}
